Initialise CC AST

theories/autosubst/CCAST.sig
@@ -1,0 +1,16 @@
+-- Universe levels and qualities
+level : Type
+cmode : Type
+
+-- Syntax
+
+cterm(var) : Type
+
+cSort : cmode -> level -> cterm
+
+cPi : level -> level -> cmode -> cmode -> cterm -> (bind cterm in cterm) -> cterm
+clam : cmode -> cterm -> (bind cterm in cterm) -> (bind cterm in cterm) -> cterm
+capp : cterm -> cterm -> cterm
+
+cbot : cterm
+cbot_elim : cmode -> cterm -> cterm -> cterm
