theories/BasicAST.v
@@ -3,3 +3,5 @@ From Coq Require Import Utf8.
 Definition level := nat.
 
 Inductive mode := mKind | mType | mGhost | mProp.
+
+Inductive cmode := cType | cProp.
