theories/autosubst/CCAST.v
@@ -1,0 +1,1260 @@
+From GhostTT.autosubst Require Import core unscoped.
+From GhostTT Require Import BasicAST.
+From Coq Require Import Setoid Morphisms Relation_Definitions.
+
+
+Module Core.
+
+Inductive cterm : Type :=
+  | var : nat -> cterm
+  | cSort : cmode -> level -> cterm
+  | cPi : level -> level -> cmode -> cmode -> cterm -> cterm -> cterm
+  | clam : cmode -> cterm -> cterm -> cterm -> cterm
+  | capp : cterm -> cterm -> cterm
+  | cbot : cterm
+  | cbot_elim : cmode -> cterm -> cterm -> cterm.
+
+Lemma congr_cSort {s0 : cmode} {s1 : level} {t0 : cmode} {t1 : level}
+  (H0 : s0 = t0) (H1 : s1 = t1) : cSort s0 s1 = cSort t0 t1.
+Proof.
+exact (eq_trans (eq_trans eq_refl (ap (fun x => cSort x s1) H0))
+         (ap (fun x => cSort t0 x) H1)).
+Qed.
+
+Lemma congr_cPi {s0 : level} {s1 : level} {s2 : cmode} {s3 : cmode}
+  {s4 : cterm} {s5 : cterm} {t0 : level} {t1 : level} {t2 : cmode}
+  {t3 : cmode} {t4 : cterm} {t5 : cterm} (H0 : s0 = t0) (H1 : s1 = t1)
+  (H2 : s2 = t2) (H3 : s3 = t3) (H4 : s4 = t4) (H5 : s5 = t5) :
+  cPi s0 s1 s2 s3 s4 s5 = cPi t0 t1 t2 t3 t4 t5.
+Proof.
+exact (eq_trans
+         (eq_trans
+            (eq_trans
+               (eq_trans
+                  (eq_trans
+                     (eq_trans eq_refl
+                        (ap (fun x => cPi x s1 s2 s3 s4 s5) H0))
+                     (ap (fun x => cPi t0 x s2 s3 s4 s5) H1))
+                  (ap (fun x => cPi t0 t1 x s3 s4 s5) H2))
+               (ap (fun x => cPi t0 t1 t2 x s4 s5) H3))
+            (ap (fun x => cPi t0 t1 t2 t3 x s5) H4))
+         (ap (fun x => cPi t0 t1 t2 t3 t4 x) H5)).
+Qed.
+
+Lemma congr_clam {s0 : cmode} {s1 : cterm} {s2 : cterm} {s3 : cterm}
+  {t0 : cmode} {t1 : cterm} {t2 : cterm} {t3 : cterm} (H0 : s0 = t0)
+  (H1 : s1 = t1) (H2 : s2 = t2) (H3 : s3 = t3) :
+  clam s0 s1 s2 s3 = clam t0 t1 t2 t3.
+Proof.
+exact (eq_trans
+         (eq_trans
+            (eq_trans (eq_trans eq_refl (ap (fun x => clam x s1 s2 s3) H0))
+               (ap (fun x => clam t0 x s2 s3) H1))
+            (ap (fun x => clam t0 t1 x s3) H2))
+         (ap (fun x => clam t0 t1 t2 x) H3)).
+Qed.
+
+Lemma congr_capp {s0 : cterm} {s1 : cterm} {t0 : cterm} {t1 : cterm}
+  (H0 : s0 = t0) (H1 : s1 = t1) : capp s0 s1 = capp t0 t1.
+Proof.
+exact (eq_trans (eq_trans eq_refl (ap (fun x => capp x s1) H0))
+         (ap (fun x => capp t0 x) H1)).
+Qed.
+
+Lemma congr_cbot : cbot = cbot.
+Proof.
+exact (eq_refl).
+Qed.
+
+Lemma congr_cbot_elim {s0 : cmode} {s1 : cterm} {s2 : cterm} {t0 : cmode}
+  {t1 : cterm} {t2 : cterm} (H0 : s0 = t0) (H1 : s1 = t1) (H2 : s2 = t2) :
+  cbot_elim s0 s1 s2 = cbot_elim t0 t1 t2.
+Proof.
+exact (eq_trans
+         (eq_trans (eq_trans eq_refl (ap (fun x => cbot_elim x s1 s2) H0))
+            (ap (fun x => cbot_elim t0 x s2) H1))
+         (ap (fun x => cbot_elim t0 t1 x) H2)).
+Qed.
+
+Lemma upRen_cterm_cterm (xi : nat -> nat) : nat -> nat.
+Proof.
+exact (up_ren xi).
+Defined.
+
+Fixpoint ren_cterm (xi_cterm : nat -> nat) (s : cterm) {struct s} : cterm :=
+  match s with
+  | var s0 => var (xi_cterm s0)
+  | cSort s0 s1 => cSort s0 s1
+  | cPi s0 s1 s2 s3 s4 s5 =>
+      cPi s0 s1 s2 s3 (ren_cterm xi_cterm s4)
+        (ren_cterm (upRen_cterm_cterm xi_cterm) s5)
+  | clam s0 s1 s2 s3 =>
+      clam s0 (ren_cterm xi_cterm s1)
+        (ren_cterm (upRen_cterm_cterm xi_cterm) s2)
+        (ren_cterm (upRen_cterm_cterm xi_cterm) s3)
+  | capp s0 s1 => capp (ren_cterm xi_cterm s0) (ren_cterm xi_cterm s1)
+  | cbot => cbot
+  | cbot_elim s0 s1 s2 =>
+      cbot_elim s0 (ren_cterm xi_cterm s1) (ren_cterm xi_cterm s2)
+  end.
+
+Lemma up_cterm_cterm (sigma : nat -> cterm) : nat -> cterm.
+Proof.
+exact (scons (var var_zero) (funcomp (ren_cterm shift) sigma)).
+Defined.
+
+Fixpoint subst_cterm (sigma_cterm : nat -> cterm) (s : cterm) {struct s} :
+cterm :=
+  match s with
+  | var s0 => sigma_cterm s0
+  | cSort s0 s1 => cSort s0 s1
+  | cPi s0 s1 s2 s3 s4 s5 =>
+      cPi s0 s1 s2 s3 (subst_cterm sigma_cterm s4)
+        (subst_cterm (up_cterm_cterm sigma_cterm) s5)
+  | clam s0 s1 s2 s3 =>
+      clam s0 (subst_cterm sigma_cterm s1)
+        (subst_cterm (up_cterm_cterm sigma_cterm) s2)
+        (subst_cterm (up_cterm_cterm sigma_cterm) s3)
+  | capp s0 s1 =>
+      capp (subst_cterm sigma_cterm s0) (subst_cterm sigma_cterm s1)
+  | cbot => cbot
+  | cbot_elim s0 s1 s2 =>
+      cbot_elim s0 (subst_cterm sigma_cterm s1) (subst_cterm sigma_cterm s2)
+  end.
+
+Lemma upId_cterm_cterm (sigma : nat -> cterm)
+  (Eq : forall x, sigma x = var x) : forall x, up_cterm_cterm sigma x = var x.
+Proof.
+exact (fun n =>
+       match n with
+       | S n' => ap (ren_cterm shift) (Eq n')
+       | O => eq_refl
+       end).
+Qed.
+
+Fixpoint idSubst_cterm (sigma_cterm : nat -> cterm)
+(Eq_cterm : forall x, sigma_cterm x = var x) (s : cterm) {struct s} :
+subst_cterm sigma_cterm s = s :=
+  match s with
+  | var s0 => Eq_cterm s0
+  | cSort s0 s1 => congr_cSort (eq_refl s0) (eq_refl s1)
+  | cPi s0 s1 s2 s3 s4 s5 =>
+      congr_cPi (eq_refl s0) (eq_refl s1) (eq_refl s2) (eq_refl s3)
+        (idSubst_cterm sigma_cterm Eq_cterm s4)
+        (idSubst_cterm (up_cterm_cterm sigma_cterm)
+           (upId_cterm_cterm _ Eq_cterm) s5)
+  | clam s0 s1 s2 s3 =>
+      congr_clam (eq_refl s0) (idSubst_cterm sigma_cterm Eq_cterm s1)
+        (idSubst_cterm (up_cterm_cterm sigma_cterm)
+           (upId_cterm_cterm _ Eq_cterm) s2)
+        (idSubst_cterm (up_cterm_cterm sigma_cterm)
+           (upId_cterm_cterm _ Eq_cterm) s3)
+  | capp s0 s1 =>
+      congr_capp (idSubst_cterm sigma_cterm Eq_cterm s0)
+        (idSubst_cterm sigma_cterm Eq_cterm s1)
+  | cbot => congr_cbot
+  | cbot_elim s0 s1 s2 =>
+      congr_cbot_elim (eq_refl s0) (idSubst_cterm sigma_cterm Eq_cterm s1)
+        (idSubst_cterm sigma_cterm Eq_cterm s2)
+  end.
+
+Lemma upExtRen_cterm_cterm (xi : nat -> nat) (zeta : nat -> nat)
+  (Eq : forall x, xi x = zeta x) :
+  forall x, upRen_cterm_cterm xi x = upRen_cterm_cterm zeta x.
+Proof.
+exact (fun n => match n with
+                | S n' => ap shift (Eq n')
+                | O => eq_refl
+                end).
+Qed.
+
+Fixpoint extRen_cterm (xi_cterm : nat -> nat) (zeta_cterm : nat -> nat)
+(Eq_cterm : forall x, xi_cterm x = zeta_cterm x) (s : cterm) {struct s} :
+ren_cterm xi_cterm s = ren_cterm zeta_cterm s :=
+  match s with
+  | var s0 => ap (var) (Eq_cterm s0)
+  | cSort s0 s1 => congr_cSort (eq_refl s0) (eq_refl s1)
+  | cPi s0 s1 s2 s3 s4 s5 =>
+      congr_cPi (eq_refl s0) (eq_refl s1) (eq_refl s2) (eq_refl s3)
+        (extRen_cterm xi_cterm zeta_cterm Eq_cterm s4)
+        (extRen_cterm (upRen_cterm_cterm xi_cterm)
+           (upRen_cterm_cterm zeta_cterm) (upExtRen_cterm_cterm _ _ Eq_cterm)
+           s5)
+  | clam s0 s1 s2 s3 =>
+      congr_clam (eq_refl s0) (extRen_cterm xi_cterm zeta_cterm Eq_cterm s1)
+        (extRen_cterm (upRen_cterm_cterm xi_cterm)
+           (upRen_cterm_cterm zeta_cterm) (upExtRen_cterm_cterm _ _ Eq_cterm)
+           s2)
+        (extRen_cterm (upRen_cterm_cterm xi_cterm)
+           (upRen_cterm_cterm zeta_cterm) (upExtRen_cterm_cterm _ _ Eq_cterm)
+           s3)
+  | capp s0 s1 =>
+      congr_capp (extRen_cterm xi_cterm zeta_cterm Eq_cterm s0)
+        (extRen_cterm xi_cterm zeta_cterm Eq_cterm s1)
+  | cbot => congr_cbot
+  | cbot_elim s0 s1 s2 =>
+      congr_cbot_elim (eq_refl s0)
+        (extRen_cterm xi_cterm zeta_cterm Eq_cterm s1)
+        (extRen_cterm xi_cterm zeta_cterm Eq_cterm s2)
+  end.
+
+Lemma upExt_cterm_cterm (sigma : nat -> cterm) (tau : nat -> cterm)
+  (Eq : forall x, sigma x = tau x) :
+  forall x, up_cterm_cterm sigma x = up_cterm_cterm tau x.
+Proof.
+exact (fun n =>
+       match n with
+       | S n' => ap (ren_cterm shift) (Eq n')
+       | O => eq_refl
+       end).
+Qed.
+
+Fixpoint ext_cterm (sigma_cterm : nat -> cterm) (tau_cterm : nat -> cterm)
+(Eq_cterm : forall x, sigma_cterm x = tau_cterm x) (s : cterm) {struct s} :
+subst_cterm sigma_cterm s = subst_cterm tau_cterm s :=
+  match s with
+  | var s0 => Eq_cterm s0
+  | cSort s0 s1 => congr_cSort (eq_refl s0) (eq_refl s1)
+  | cPi s0 s1 s2 s3 s4 s5 =>
+      congr_cPi (eq_refl s0) (eq_refl s1) (eq_refl s2) (eq_refl s3)
+        (ext_cterm sigma_cterm tau_cterm Eq_cterm s4)
+        (ext_cterm (up_cterm_cterm sigma_cterm) (up_cterm_cterm tau_cterm)
+           (upExt_cterm_cterm _ _ Eq_cterm) s5)
+  | clam s0 s1 s2 s3 =>
+      congr_clam (eq_refl s0) (ext_cterm sigma_cterm tau_cterm Eq_cterm s1)
+        (ext_cterm (up_cterm_cterm sigma_cterm) (up_cterm_cterm tau_cterm)
+           (upExt_cterm_cterm _ _ Eq_cterm) s2)
+        (ext_cterm (up_cterm_cterm sigma_cterm) (up_cterm_cterm tau_cterm)
+           (upExt_cterm_cterm _ _ Eq_cterm) s3)
+  | capp s0 s1 =>
+      congr_capp (ext_cterm sigma_cterm tau_cterm Eq_cterm s0)
+        (ext_cterm sigma_cterm tau_cterm Eq_cterm s1)
+  | cbot => congr_cbot
+  | cbot_elim s0 s1 s2 =>
+      congr_cbot_elim (eq_refl s0)
+        (ext_cterm sigma_cterm tau_cterm Eq_cterm s1)
+        (ext_cterm sigma_cterm tau_cterm Eq_cterm s2)
+  end.
+
+Lemma up_ren_ren_cterm_cterm (xi : nat -> nat) (zeta : nat -> nat)
+  (rho : nat -> nat) (Eq : forall x, funcomp zeta xi x = rho x) :
+  forall x,
+  funcomp (upRen_cterm_cterm zeta) (upRen_cterm_cterm xi) x =
+  upRen_cterm_cterm rho x.
+Proof.
+exact (up_ren_ren xi zeta rho Eq).
+Qed.
+
+Fixpoint compRenRen_cterm (xi_cterm : nat -> nat) (zeta_cterm : nat -> nat)
+(rho_cterm : nat -> nat)
+(Eq_cterm : forall x, funcomp zeta_cterm xi_cterm x = rho_cterm x)
+(s : cterm) {struct s} :
+ren_cterm zeta_cterm (ren_cterm xi_cterm s) = ren_cterm rho_cterm s :=
+  match s with
+  | var s0 => ap (var) (Eq_cterm s0)
+  | cSort s0 s1 => congr_cSort (eq_refl s0) (eq_refl s1)
+  | cPi s0 s1 s2 s3 s4 s5 =>
+      congr_cPi (eq_refl s0) (eq_refl s1) (eq_refl s2) (eq_refl s3)
+        (compRenRen_cterm xi_cterm zeta_cterm rho_cterm Eq_cterm s4)
+        (compRenRen_cterm (upRen_cterm_cterm xi_cterm)
+           (upRen_cterm_cterm zeta_cterm) (upRen_cterm_cterm rho_cterm)
+           (up_ren_ren _ _ _ Eq_cterm) s5)
+  | clam s0 s1 s2 s3 =>
+      congr_clam (eq_refl s0)
+        (compRenRen_cterm xi_cterm zeta_cterm rho_cterm Eq_cterm s1)
+        (compRenRen_cterm (upRen_cterm_cterm xi_cterm)
+           (upRen_cterm_cterm zeta_cterm) (upRen_cterm_cterm rho_cterm)
+           (up_ren_ren _ _ _ Eq_cterm) s2)
+        (compRenRen_cterm (upRen_cterm_cterm xi_cterm)
+           (upRen_cterm_cterm zeta_cterm) (upRen_cterm_cterm rho_cterm)
+           (up_ren_ren _ _ _ Eq_cterm) s3)
+  | capp s0 s1 =>
+      congr_capp (compRenRen_cterm xi_cterm zeta_cterm rho_cterm Eq_cterm s0)
+        (compRenRen_cterm xi_cterm zeta_cterm rho_cterm Eq_cterm s1)
+  | cbot => congr_cbot
+  | cbot_elim s0 s1 s2 =>
+      congr_cbot_elim (eq_refl s0)
+        (compRenRen_cterm xi_cterm zeta_cterm rho_cterm Eq_cterm s1)
+        (compRenRen_cterm xi_cterm zeta_cterm rho_cterm Eq_cterm s2)
+  end.
+
+Lemma up_ren_subst_cterm_cterm (xi : nat -> nat) (tau : nat -> cterm)
+  (theta : nat -> cterm) (Eq : forall x, funcomp tau xi x = theta x) :
+  forall x,
+  funcomp (up_cterm_cterm tau) (upRen_cterm_cterm xi) x =
+  up_cterm_cterm theta x.
+Proof.
+exact (fun n =>
+       match n with
+       | S n' => ap (ren_cterm shift) (Eq n')
+       | O => eq_refl
+       end).
+Qed.
+
+Fixpoint compRenSubst_cterm (xi_cterm : nat -> nat)
+(tau_cterm : nat -> cterm) (theta_cterm : nat -> cterm)
+(Eq_cterm : forall x, funcomp tau_cterm xi_cterm x = theta_cterm x)
+(s : cterm) {struct s} :
+subst_cterm tau_cterm (ren_cterm xi_cterm s) = subst_cterm theta_cterm s :=
+  match s with
+  | var s0 => Eq_cterm s0
+  | cSort s0 s1 => congr_cSort (eq_refl s0) (eq_refl s1)
+  | cPi s0 s1 s2 s3 s4 s5 =>
+      congr_cPi (eq_refl s0) (eq_refl s1) (eq_refl s2) (eq_refl s3)
+        (compRenSubst_cterm xi_cterm tau_cterm theta_cterm Eq_cterm s4)
+        (compRenSubst_cterm (upRen_cterm_cterm xi_cterm)
+           (up_cterm_cterm tau_cterm) (up_cterm_cterm theta_cterm)
+           (up_ren_subst_cterm_cterm _ _ _ Eq_cterm) s5)
+  | clam s0 s1 s2 s3 =>
+      congr_clam (eq_refl s0)
+        (compRenSubst_cterm xi_cterm tau_cterm theta_cterm Eq_cterm s1)
+        (compRenSubst_cterm (upRen_cterm_cterm xi_cterm)
+           (up_cterm_cterm tau_cterm) (up_cterm_cterm theta_cterm)
+           (up_ren_subst_cterm_cterm _ _ _ Eq_cterm) s2)
+        (compRenSubst_cterm (upRen_cterm_cterm xi_cterm)
+           (up_cterm_cterm tau_cterm) (up_cterm_cterm theta_cterm)
+           (up_ren_subst_cterm_cterm _ _ _ Eq_cterm) s3)
+  | capp s0 s1 =>
+      congr_capp
+        (compRenSubst_cterm xi_cterm tau_cterm theta_cterm Eq_cterm s0)
+        (compRenSubst_cterm xi_cterm tau_cterm theta_cterm Eq_cterm s1)
+  | cbot => congr_cbot
+  | cbot_elim s0 s1 s2 =>
+      congr_cbot_elim (eq_refl s0)
+        (compRenSubst_cterm xi_cterm tau_cterm theta_cterm Eq_cterm s1)
+        (compRenSubst_cterm xi_cterm tau_cterm theta_cterm Eq_cterm s2)
+  end.
+
+Lemma up_subst_ren_cterm_cterm (sigma : nat -> cterm)
+  (zeta_cterm : nat -> nat) (theta : nat -> cterm)
+  (Eq : forall x, funcomp (ren_cterm zeta_cterm) sigma x = theta x) :
+  forall x,
+  funcomp (ren_cterm (upRen_cterm_cterm zeta_cterm)) (up_cterm_cterm sigma) x =
+  up_cterm_cterm theta x.
+Proof.
+exact (fun n =>
+       match n with
+       | S n' =>
+           eq_trans
+             (compRenRen_cterm shift (upRen_cterm_cterm zeta_cterm)
+                (funcomp shift zeta_cterm) (fun x => eq_refl) (sigma n'))
+             (eq_trans
+                (eq_sym
+                   (compRenRen_cterm zeta_cterm shift
+                      (funcomp shift zeta_cterm) (fun x => eq_refl)
+                      (sigma n'))) (ap (ren_cterm shift) (Eq n')))
+       | O => eq_refl
+       end).
+Qed.
+
+Fixpoint compSubstRen_cterm (sigma_cterm : nat -> cterm)
+(zeta_cterm : nat -> nat) (theta_cterm : nat -> cterm)
+(Eq_cterm : forall x,
+            funcomp (ren_cterm zeta_cterm) sigma_cterm x = theta_cterm x)
+(s : cterm) {struct s} :
+ren_cterm zeta_cterm (subst_cterm sigma_cterm s) = subst_cterm theta_cterm s
+:=
+  match s with
+  | var s0 => Eq_cterm s0
+  | cSort s0 s1 => congr_cSort (eq_refl s0) (eq_refl s1)
+  | cPi s0 s1 s2 s3 s4 s5 =>
+      congr_cPi (eq_refl s0) (eq_refl s1) (eq_refl s2) (eq_refl s3)
+        (compSubstRen_cterm sigma_cterm zeta_cterm theta_cterm Eq_cterm s4)
+        (compSubstRen_cterm (up_cterm_cterm sigma_cterm)
+           (upRen_cterm_cterm zeta_cterm) (up_cterm_cterm theta_cterm)
+           (up_subst_ren_cterm_cterm _ _ _ Eq_cterm) s5)
+  | clam s0 s1 s2 s3 =>
+      congr_clam (eq_refl s0)
+        (compSubstRen_cterm sigma_cterm zeta_cterm theta_cterm Eq_cterm s1)
+        (compSubstRen_cterm (up_cterm_cterm sigma_cterm)
+           (upRen_cterm_cterm zeta_cterm) (up_cterm_cterm theta_cterm)
+           (up_subst_ren_cterm_cterm _ _ _ Eq_cterm) s2)
+        (compSubstRen_cterm (up_cterm_cterm sigma_cterm)
+           (upRen_cterm_cterm zeta_cterm) (up_cterm_cterm theta_cterm)
+           (up_subst_ren_cterm_cterm _ _ _ Eq_cterm) s3)
+  | capp s0 s1 =>
+      congr_capp
+        (compSubstRen_cterm sigma_cterm zeta_cterm theta_cterm Eq_cterm s0)
+        (compSubstRen_cterm sigma_cterm zeta_cterm theta_cterm Eq_cterm s1)
+  | cbot => congr_cbot
+  | cbot_elim s0 s1 s2 =>
+      congr_cbot_elim (eq_refl s0)
+        (compSubstRen_cterm sigma_cterm zeta_cterm theta_cterm Eq_cterm s1)
+        (compSubstRen_cterm sigma_cterm zeta_cterm theta_cterm Eq_cterm s2)
+  end.
+
+Lemma up_subst_subst_cterm_cterm (sigma : nat -> cterm)
+  (tau_cterm : nat -> cterm) (theta : nat -> cterm)
+  (Eq : forall x, funcomp (subst_cterm tau_cterm) sigma x = theta x) :
+  forall x,
+  funcomp (subst_cterm (up_cterm_cterm tau_cterm)) (up_cterm_cterm sigma) x =
+  up_cterm_cterm theta x.
+Proof.
+exact (fun n =>
+       match n with
+       | S n' =>
+           eq_trans
+             (compRenSubst_cterm shift (up_cterm_cterm tau_cterm)
+                (funcomp (up_cterm_cterm tau_cterm) shift) (fun x => eq_refl)
+                (sigma n'))
+             (eq_trans
+                (eq_sym
+                   (compSubstRen_cterm tau_cterm shift
+                      (funcomp (ren_cterm shift) tau_cterm)
+                      (fun x => eq_refl) (sigma n')))
+                (ap (ren_cterm shift) (Eq n')))
+       | O => eq_refl
+       end).
+Qed.
+
+Fixpoint compSubstSubst_cterm (sigma_cterm : nat -> cterm)
+(tau_cterm : nat -> cterm) (theta_cterm : nat -> cterm)
+(Eq_cterm : forall x,
+            funcomp (subst_cterm tau_cterm) sigma_cterm x = theta_cterm x)
+(s : cterm) {struct s} :
+subst_cterm tau_cterm (subst_cterm sigma_cterm s) = subst_cterm theta_cterm s
+:=
+  match s with
+  | var s0 => Eq_cterm s0
+  | cSort s0 s1 => congr_cSort (eq_refl s0) (eq_refl s1)
+  | cPi s0 s1 s2 s3 s4 s5 =>
+      congr_cPi (eq_refl s0) (eq_refl s1) (eq_refl s2) (eq_refl s3)
+        (compSubstSubst_cterm sigma_cterm tau_cterm theta_cterm Eq_cterm s4)
+        (compSubstSubst_cterm (up_cterm_cterm sigma_cterm)
+           (up_cterm_cterm tau_cterm) (up_cterm_cterm theta_cterm)
+           (up_subst_subst_cterm_cterm _ _ _ Eq_cterm) s5)
+  | clam s0 s1 s2 s3 =>
+      congr_clam (eq_refl s0)
+        (compSubstSubst_cterm sigma_cterm tau_cterm theta_cterm Eq_cterm s1)
+        (compSubstSubst_cterm (up_cterm_cterm sigma_cterm)
+           (up_cterm_cterm tau_cterm) (up_cterm_cterm theta_cterm)
+           (up_subst_subst_cterm_cterm _ _ _ Eq_cterm) s2)
+        (compSubstSubst_cterm (up_cterm_cterm sigma_cterm)
+           (up_cterm_cterm tau_cterm) (up_cterm_cterm theta_cterm)
+           (up_subst_subst_cterm_cterm _ _ _ Eq_cterm) s3)
+  | capp s0 s1 =>
+      congr_capp
+        (compSubstSubst_cterm sigma_cterm tau_cterm theta_cterm Eq_cterm s0)
+        (compSubstSubst_cterm sigma_cterm tau_cterm theta_cterm Eq_cterm s1)
+  | cbot => congr_cbot
+  | cbot_elim s0 s1 s2 =>
+      congr_cbot_elim (eq_refl s0)
+        (compSubstSubst_cterm sigma_cterm tau_cterm theta_cterm Eq_cterm s1)
+        (compSubstSubst_cterm sigma_cterm tau_cterm theta_cterm Eq_cterm s2)
+  end.
+
+Lemma renRen_cterm (xi_cterm : nat -> nat) (zeta_cterm : nat -> nat)
+  (s : cterm) :
+  ren_cterm zeta_cterm (ren_cterm xi_cterm s) =
+  ren_cterm (funcomp zeta_cterm xi_cterm) s.
+Proof.
+exact (compRenRen_cterm xi_cterm zeta_cterm _ (fun n => eq_refl) s).
+Qed.
+
+Lemma renRen'_cterm_pointwise (xi_cterm : nat -> nat)
+  (zeta_cterm : nat -> nat) :
+  pointwise_relation _ eq
+    (funcomp (ren_cterm zeta_cterm) (ren_cterm xi_cterm))
+    (ren_cterm (funcomp zeta_cterm xi_cterm)).
+Proof.
+exact (fun s => compRenRen_cterm xi_cterm zeta_cterm _ (fun n => eq_refl) s).
+Qed.
+
+Lemma renSubst_cterm (xi_cterm : nat -> nat) (tau_cterm : nat -> cterm)
+  (s : cterm) :
+  subst_cterm tau_cterm (ren_cterm xi_cterm s) =
+  subst_cterm (funcomp tau_cterm xi_cterm) s.
+Proof.
+exact (compRenSubst_cterm xi_cterm tau_cterm _ (fun n => eq_refl) s).
+Qed.
+
+Lemma renSubst_cterm_pointwise (xi_cterm : nat -> nat)
+  (tau_cterm : nat -> cterm) :
+  pointwise_relation _ eq
+    (funcomp (subst_cterm tau_cterm) (ren_cterm xi_cterm))
+    (subst_cterm (funcomp tau_cterm xi_cterm)).
+Proof.
+exact (fun s => compRenSubst_cterm xi_cterm tau_cterm _ (fun n => eq_refl) s).
+Qed.
+
+Lemma substRen_cterm (sigma_cterm : nat -> cterm) (zeta_cterm : nat -> nat)
+  (s : cterm) :
+  ren_cterm zeta_cterm (subst_cterm sigma_cterm s) =
+  subst_cterm (funcomp (ren_cterm zeta_cterm) sigma_cterm) s.
+Proof.
+exact (compSubstRen_cterm sigma_cterm zeta_cterm _ (fun n => eq_refl) s).
+Qed.
+
+Lemma substRen_cterm_pointwise (sigma_cterm : nat -> cterm)
+  (zeta_cterm : nat -> nat) :
+  pointwise_relation _ eq
+    (funcomp (ren_cterm zeta_cterm) (subst_cterm sigma_cterm))
+    (subst_cterm (funcomp (ren_cterm zeta_cterm) sigma_cterm)).
+Proof.
+exact (fun s =>
+       compSubstRen_cterm sigma_cterm zeta_cterm _ (fun n => eq_refl) s).
+Qed.
+
+Lemma substSubst_cterm (sigma_cterm : nat -> cterm)
+  (tau_cterm : nat -> cterm) (s : cterm) :
+  subst_cterm tau_cterm (subst_cterm sigma_cterm s) =
+  subst_cterm (funcomp (subst_cterm tau_cterm) sigma_cterm) s.
+Proof.
+exact (compSubstSubst_cterm sigma_cterm tau_cterm _ (fun n => eq_refl) s).
+Qed.
+
+Lemma substSubst_cterm_pointwise (sigma_cterm : nat -> cterm)
+  (tau_cterm : nat -> cterm) :
+  pointwise_relation _ eq
+    (funcomp (subst_cterm tau_cterm) (subst_cterm sigma_cterm))
+    (subst_cterm (funcomp (subst_cterm tau_cterm) sigma_cterm)).
+Proof.
+exact (fun s =>
+       compSubstSubst_cterm sigma_cterm tau_cterm _ (fun n => eq_refl) s).
+Qed.
+
+Lemma rinstInst_up_cterm_cterm (xi : nat -> nat) (sigma : nat -> cterm)
+  (Eq : forall x, funcomp (var) xi x = sigma x) :
+  forall x, funcomp (var) (upRen_cterm_cterm xi) x = up_cterm_cterm sigma x.
+Proof.
+exact (fun n =>
+       match n with
+       | S n' => ap (ren_cterm shift) (Eq n')
+       | O => eq_refl
+       end).
+Qed.
+
+Fixpoint rinst_inst_cterm (xi_cterm : nat -> nat)
+(sigma_cterm : nat -> cterm)
+(Eq_cterm : forall x, funcomp (var) xi_cterm x = sigma_cterm x) (s : cterm)
+{struct s} : ren_cterm xi_cterm s = subst_cterm sigma_cterm s :=
+  match s with
+  | var s0 => Eq_cterm s0
+  | cSort s0 s1 => congr_cSort (eq_refl s0) (eq_refl s1)
+  | cPi s0 s1 s2 s3 s4 s5 =>
+      congr_cPi (eq_refl s0) (eq_refl s1) (eq_refl s2) (eq_refl s3)
+        (rinst_inst_cterm xi_cterm sigma_cterm Eq_cterm s4)
+        (rinst_inst_cterm (upRen_cterm_cterm xi_cterm)
+           (up_cterm_cterm sigma_cterm)
+           (rinstInst_up_cterm_cterm _ _ Eq_cterm) s5)
+  | clam s0 s1 s2 s3 =>
+      congr_clam (eq_refl s0)
+        (rinst_inst_cterm xi_cterm sigma_cterm Eq_cterm s1)
+        (rinst_inst_cterm (upRen_cterm_cterm xi_cterm)
+           (up_cterm_cterm sigma_cterm)
+           (rinstInst_up_cterm_cterm _ _ Eq_cterm) s2)
+        (rinst_inst_cterm (upRen_cterm_cterm xi_cterm)
+           (up_cterm_cterm sigma_cterm)
+           (rinstInst_up_cterm_cterm _ _ Eq_cterm) s3)
+  | capp s0 s1 =>
+      congr_capp (rinst_inst_cterm xi_cterm sigma_cterm Eq_cterm s0)
+        (rinst_inst_cterm xi_cterm sigma_cterm Eq_cterm s1)
+  | cbot => congr_cbot
+  | cbot_elim s0 s1 s2 =>
+      congr_cbot_elim (eq_refl s0)
+        (rinst_inst_cterm xi_cterm sigma_cterm Eq_cterm s1)
+        (rinst_inst_cterm xi_cterm sigma_cterm Eq_cterm s2)
+  end.
+
+Lemma rinstInst'_cterm (xi_cterm : nat -> nat) (s : cterm) :
+  ren_cterm xi_cterm s = subst_cterm (funcomp (var) xi_cterm) s.
+Proof.
+exact (rinst_inst_cterm xi_cterm _ (fun n => eq_refl) s).
+Qed.
+
+Lemma rinstInst'_cterm_pointwise (xi_cterm : nat -> nat) :
+  pointwise_relation _ eq (ren_cterm xi_cterm)
+    (subst_cterm (funcomp (var) xi_cterm)).
+Proof.
+exact (fun s => rinst_inst_cterm xi_cterm _ (fun n => eq_refl) s).
+Qed.
+
+Lemma instId'_cterm (s : cterm) : subst_cterm (var) s = s.
+Proof.
+exact (idSubst_cterm (var) (fun n => eq_refl) s).
+Qed.
+
+Lemma instId'_cterm_pointwise :
+  pointwise_relation _ eq (subst_cterm (var)) id.
+Proof.
+exact (fun s => idSubst_cterm (var) (fun n => eq_refl) s).
+Qed.
+
+Lemma rinstId'_cterm (s : cterm) : ren_cterm id s = s.
+Proof.
+exact (eq_ind_r (fun t => t = s) (instId'_cterm s) (rinstInst'_cterm id s)).
+Qed.
+
+Lemma rinstId'_cterm_pointwise : pointwise_relation _ eq (@ren_cterm id) id.
+Proof.
+exact (fun s =>
+       eq_ind_r (fun t => t = s) (instId'_cterm s) (rinstInst'_cterm id s)).
+Qed.
+
+Lemma varL'_cterm (sigma_cterm : nat -> cterm) (x : nat) :
+  subst_cterm sigma_cterm (var x) = sigma_cterm x.
+Proof.
+exact (eq_refl).
+Qed.
+
+Lemma varL'_cterm_pointwise (sigma_cterm : nat -> cterm) :
+  pointwise_relation _ eq (funcomp (subst_cterm sigma_cterm) (var))
+    sigma_cterm.
+Proof.
+exact (fun x => eq_refl).
+Qed.
+
+Lemma varLRen'_cterm (xi_cterm : nat -> nat) (x : nat) :
+  ren_cterm xi_cterm (var x) = var (xi_cterm x).
+Proof.
+exact (eq_refl).
+Qed.
+
+Lemma varLRen'_cterm_pointwise (xi_cterm : nat -> nat) :
+  pointwise_relation _ eq (funcomp (ren_cterm xi_cterm) (var))
+    (funcomp (var) xi_cterm).
+Proof.
+exact (fun x => eq_refl).
+Qed.
+
+Class Up_cterm X Y :=
+    up_cterm : X -> Y.
+
+#[global]Instance Subst_cterm : (Subst1 _ _ _) := @subst_cterm.
+
+#[global]
+Instance Up_cterm_cterm : (Up_cterm _ _) := @up_cterm_cterm.
+
+#[global]Instance Ren_cterm : (Ren1 _ _ _) := @ren_cterm.
+
+#[global]
+Instance VarInstance_cterm : (Var _ _) := @var.
+
+Notation "[ sigma_cterm ]" := (subst_cterm sigma_cterm)
+  ( at level 1, left associativity, only printing) : fscope.
+
+Notation "s [ sigma_cterm ]" := (subst_cterm sigma_cterm s)
+  ( at level 7, left associativity, only printing) : subst_scope.
+
+Notation "↑__cterm" := up_cterm (only printing) : subst_scope.
+
+Notation "↑__cterm" := up_cterm_cterm (only printing) : subst_scope.
+
+Notation "⟨ xi_cterm ⟩" := (ren_cterm xi_cterm)
+  ( at level 1, left associativity, only printing) : fscope.
+
+Notation "s ⟨ xi_cterm ⟩" := (ren_cterm xi_cterm s)
+  ( at level 7, left associativity, only printing) : subst_scope.
+
+Notation "'var'" := var ( at level 1, only printing) : subst_scope.
+
+Notation "x '__cterm'" := (@ids _ _ VarInstance_cterm x)
+  ( at level 5, format "x __cterm", only printing) : subst_scope.
+
+Notation "x '__cterm'" := (var x) ( at level 5, format "x __cterm") :
+  subst_scope.
+
+#[global]
+Instance subst_cterm_morphism :
+ (Proper (respectful (pointwise_relation _ eq) (respectful eq eq))
+    (@subst_cterm)).
+Proof.
+exact (fun f_cterm g_cterm Eq_cterm s t Eq_st =>
+       eq_ind s (fun t' => subst_cterm f_cterm s = subst_cterm g_cterm t')
+         (ext_cterm f_cterm g_cterm Eq_cterm s) t Eq_st).
+Qed.
+
+#[global]
+Instance subst_cterm_morphism2 :
+ (Proper (respectful (pointwise_relation _ eq) (pointwise_relation _ eq))
+    (@subst_cterm)).
+Proof.
+exact (fun f_cterm g_cterm Eq_cterm s => ext_cterm f_cterm g_cterm Eq_cterm s).
+Qed.
+
+#[global]
+Instance ren_cterm_morphism :
+ (Proper (respectful (pointwise_relation _ eq) (respectful eq eq))
+    (@ren_cterm)).
+Proof.
+exact (fun f_cterm g_cterm Eq_cterm s t Eq_st =>
+       eq_ind s (fun t' => ren_cterm f_cterm s = ren_cterm g_cterm t')
+         (extRen_cterm f_cterm g_cterm Eq_cterm s) t Eq_st).
+Qed.
+
+#[global]
+Instance ren_cterm_morphism2 :
+ (Proper (respectful (pointwise_relation _ eq) (pointwise_relation _ eq))
+    (@ren_cterm)).
+Proof.
+exact (fun f_cterm g_cterm Eq_cterm s =>
+       extRen_cterm f_cterm g_cterm Eq_cterm s).
+Qed.
+
+Ltac auto_unfold := repeat
+                     unfold VarInstance_cterm, Var, ids, Ren_cterm, Ren1,
+                      ren1, Up_cterm_cterm, Up_cterm, up_cterm, Subst_cterm,
+                      Subst1, subst1.
+
+Tactic Notation "auto_unfold" "in" "*" := repeat
+                                           unfold VarInstance_cterm, Var,
+                                            ids, Ren_cterm, Ren1, ren1,
+                                            Up_cterm_cterm, Up_cterm,
+                                            up_cterm, Subst_cterm, Subst1,
+                                            subst1 in *.
+
+Ltac asimpl' := repeat (first
+                 [ progress setoid_rewrite substSubst_cterm_pointwise
+                 | progress setoid_rewrite substSubst_cterm
+                 | progress setoid_rewrite substRen_cterm_pointwise
+                 | progress setoid_rewrite substRen_cterm
+                 | progress setoid_rewrite renSubst_cterm_pointwise
+                 | progress setoid_rewrite renSubst_cterm
+                 | progress setoid_rewrite renRen'_cterm_pointwise
+                 | progress setoid_rewrite renRen_cterm
+                 | progress setoid_rewrite varLRen'_cterm_pointwise
+                 | progress setoid_rewrite varLRen'_cterm
+                 | progress setoid_rewrite varL'_cterm_pointwise
+                 | progress setoid_rewrite varL'_cterm
+                 | progress setoid_rewrite rinstId'_cterm_pointwise
+                 | progress setoid_rewrite rinstId'_cterm
+                 | progress setoid_rewrite instId'_cterm_pointwise
+                 | progress setoid_rewrite instId'_cterm
+                 | progress unfold up_cterm_cterm, upRen_cterm_cterm, up_ren
+                 | progress cbn[subst_cterm ren_cterm]
+                 | progress fsimpl ]).
+
+Ltac asimpl := check_no_evars;
+                repeat
+                 unfold VarInstance_cterm, Var, ids, Ren_cterm, Ren1, ren1,
+                  Up_cterm_cterm, Up_cterm, up_cterm, Subst_cterm, Subst1,
+                  subst1 in *; asimpl'; minimize.
+
+Tactic Notation "asimpl" "in" hyp(J) := revert J; asimpl; intros J.
+
+Tactic Notation "auto_case" := auto_case ltac:(asimpl; cbn; eauto).
+
+Ltac substify := auto_unfold; try setoid_rewrite rinstInst'_cterm_pointwise;
+                  try setoid_rewrite rinstInst'_cterm.
+
+Ltac renamify := auto_unfold;
+                  try setoid_rewrite_left rinstInst'_cterm_pointwise;
+                  try setoid_rewrite_left rinstInst'_cterm.
+
+End Core.
+
+Module Allfv.
+
+Import
+Core.
+
+Lemma upAllfv_cterm_cterm (p : nat -> Prop) : nat -> Prop.
+Proof.
+exact (up_allfv p).
+Defined.
+
+Fixpoint allfv_cterm (p_cterm : nat -> Prop) (s : cterm) {struct s} : Prop :=
+  match s with
+  | var s0 => p_cterm s0
+  | cSort s0 s1 => and True (and True True)
+  | cPi s0 s1 s2 s3 s4 s5 =>
+      and True
+        (and True
+           (and True
+              (and True
+                 (and (allfv_cterm p_cterm s4)
+                    (and (allfv_cterm (upAllfv_cterm_cterm p_cterm) s5) True)))))
+  | clam s0 s1 s2 s3 =>
+      and True
+        (and (allfv_cterm p_cterm s1)
+           (and (allfv_cterm (upAllfv_cterm_cterm p_cterm) s2)
+              (and (allfv_cterm (upAllfv_cterm_cterm p_cterm) s3) True)))
+  | capp s0 s1 =>
+      and (allfv_cterm p_cterm s0) (and (allfv_cterm p_cterm s1) True)
+  | cbot => True
+  | cbot_elim s0 s1 s2 =>
+      and True
+        (and (allfv_cterm p_cterm s1) (and (allfv_cterm p_cterm s2) True))
+  end.
+
+Lemma upAllfvTriv_cterm_cterm {p : nat -> Prop} (H : forall x, p x) :
+  forall x, upAllfv_cterm_cterm p x.
+Proof.
+exact (fun x => match x with
+                | S n' => H n'
+                | O => I
+                end).
+Qed.
+
+Fixpoint allfvTriv_cterm (p_cterm : nat -> Prop)
+(H_cterm : forall x, p_cterm x) (s : cterm) {struct s} :
+allfv_cterm p_cterm s :=
+  match s with
+  | var s0 => H_cterm s0
+  | cSort s0 s1 => conj I (conj I I)
+  | cPi s0 s1 s2 s3 s4 s5 =>
+      conj I
+        (conj I
+           (conj I
+              (conj I
+                 (conj (allfvTriv_cterm p_cterm H_cterm s4)
+                    (conj
+                       (allfvTriv_cterm (upAllfv_cterm_cterm p_cterm)
+                          (upAllfvTriv_cterm_cterm H_cterm) s5) I)))))
+  | clam s0 s1 s2 s3 =>
+      conj I
+        (conj (allfvTriv_cterm p_cterm H_cterm s1)
+           (conj
+              (allfvTriv_cterm (upAllfv_cterm_cterm p_cterm)
+                 (upAllfvTriv_cterm_cterm H_cterm) s2)
+              (conj
+                 (allfvTriv_cterm (upAllfv_cterm_cterm p_cterm)
+                    (upAllfvTriv_cterm_cterm H_cterm) s3) I)))
+  | capp s0 s1 =>
+      conj (allfvTriv_cterm p_cterm H_cterm s0)
+        (conj (allfvTriv_cterm p_cterm H_cterm s1) I)
+  | cbot => I
+  | cbot_elim s0 s1 s2 =>
+      conj I
+        (conj (allfvTriv_cterm p_cterm H_cterm s1)
+           (conj (allfvTriv_cterm p_cterm H_cterm s2) I))
+  end.
+
+Lemma upAllfvImpl_cterm_cterm {p : nat -> Prop} {q : nat -> Prop}
+  (H : forall x, p x -> q x) :
+  forall x, upAllfv_cterm_cterm p x -> upAllfv_cterm_cterm q x.
+Proof.
+exact (fun x => match x with
+                | S n' => H n'
+                | O => fun Hp => Hp
+                end).
+Qed.
+
+Fixpoint allfvImpl_cterm (p_cterm : nat -> Prop) (q_cterm : nat -> Prop)
+(H_cterm : forall x, p_cterm x -> q_cterm x) (s : cterm) {struct s} :
+allfv_cterm p_cterm s -> allfv_cterm q_cterm s :=
+  match s with
+  | var s0 => fun HP => H_cterm s0 HP
+  | cSort s0 s1 => fun HP => conj I (conj I I)
+  | cPi s0 s1 s2 s3 s4 s5 =>
+      fun HP =>
+      conj I
+        (conj I
+           (conj I
+              (conj I
+                 (conj
+                    (allfvImpl_cterm p_cterm q_cterm H_cterm s4
+                       match HP with
+                       | conj _ HP =>
+                           match HP with
+                           | conj _ HP =>
+                               match HP with
+                               | conj _ HP =>
+                                   match HP with
+                                   | conj _ HP =>
+                                       match HP with
+                                       | conj HP _ => HP
+                                       end
+                                   end
+                               end
+                           end
+                       end)
+                    (conj
+                       (allfvImpl_cterm (upAllfv_cterm_cterm p_cterm)
+                          (upAllfv_cterm_cterm q_cterm)
+                          (upAllfvImpl_cterm_cterm H_cterm) s5
+                          match HP with
+                          | conj _ HP =>
+                              match HP with
+                              | conj _ HP =>
+                                  match HP with
+                                  | conj _ HP =>
+                                      match HP with
+                                      | conj _ HP =>
+                                          match HP with
+                                          | conj _ HP =>
+                                              match HP with
+                                              | conj HP _ => HP
+                                              end
+                                          end
+                                      end
+                                  end
+                              end
+                          end) I)))))
+  | clam s0 s1 s2 s3 =>
+      fun HP =>
+      conj I
+        (conj
+           (allfvImpl_cterm p_cterm q_cterm H_cterm s1
+              match HP with
+              | conj _ HP => match HP with
+                             | conj HP _ => HP
+                             end
+              end)
+           (conj
+              (allfvImpl_cterm (upAllfv_cterm_cterm p_cterm)
+                 (upAllfv_cterm_cterm q_cterm)
+                 (upAllfvImpl_cterm_cterm H_cterm) s2
+                 match HP with
+                 | conj _ HP =>
+                     match HP with
+                     | conj _ HP => match HP with
+                                    | conj HP _ => HP
+                                    end
+                     end
+                 end)
+              (conj
+                 (allfvImpl_cterm (upAllfv_cterm_cterm p_cterm)
+                    (upAllfv_cterm_cterm q_cterm)
+                    (upAllfvImpl_cterm_cterm H_cterm) s3
+                    match HP with
+                    | conj _ HP =>
+                        match HP with
+                        | conj _ HP =>
+                            match HP with
+                            | conj _ HP =>
+                                match HP with
+                                | conj HP _ => HP
+                                end
+                            end
+                        end
+                    end) I)))
+  | capp s0 s1 =>
+      fun HP =>
+      conj
+        (allfvImpl_cterm p_cterm q_cterm H_cterm s0
+           match HP with
+           | conj HP _ => HP
+           end)
+        (conj
+           (allfvImpl_cterm p_cterm q_cterm H_cterm s1
+              match HP with
+              | conj _ HP => match HP with
+                             | conj HP _ => HP
+                             end
+              end) I)
+  | cbot => fun HP => I
+  | cbot_elim s0 s1 s2 =>
+      fun HP =>
+      conj I
+        (conj
+           (allfvImpl_cterm p_cterm q_cterm H_cterm s1
+              match HP with
+              | conj _ HP => match HP with
+                             | conj HP _ => HP
+                             end
+              end)
+           (conj
+              (allfvImpl_cterm p_cterm q_cterm H_cterm s2
+                 match HP with
+                 | conj _ HP =>
+                     match HP with
+                     | conj _ HP => match HP with
+                                    | conj HP _ => HP
+                                    end
+                     end
+                 end) I))
+  end.
+
+Lemma upAllfvRenL_cterm_cterm (p : nat -> Prop) (xi : nat -> nat) :
+  forall x,
+  upAllfv_cterm_cterm p (upRen_cterm_cterm xi x) ->
+  upAllfv_cterm_cterm (funcomp p xi) x.
+Proof.
+exact (fun x => match x with
+                | S n' => fun i => i
+                | O => fun H => H
+                end).
+Qed.
+
+Fixpoint allfvRenL_cterm (p_cterm : nat -> Prop) (xi_cterm : nat -> nat)
+(s : cterm) {struct s} :
+allfv_cterm p_cterm (ren_cterm xi_cterm s) ->
+allfv_cterm (funcomp p_cterm xi_cterm) s :=
+  match s with
+  | var s0 => fun H => H
+  | cSort s0 s1 => fun H => conj I (conj I I)
+  | cPi s0 s1 s2 s3 s4 s5 =>
+      fun H =>
+      conj I
+        (conj I
+           (conj I
+              (conj I
+                 (conj
+                    (allfvRenL_cterm p_cterm xi_cterm s4
+                       match H with
+                       | conj _ H =>
+                           match H with
+                           | conj _ H =>
+                               match H with
+                               | conj _ H =>
+                                   match H with
+                                   | conj _ H =>
+                                       match H with
+                                       | conj H _ => H
+                                       end
+                                   end
+                               end
+                           end
+                       end)
+                    (conj
+                       (allfvImpl_cterm _ _
+                          (upAllfvRenL_cterm_cterm p_cterm xi_cterm) s5
+                          (allfvRenL_cterm (upAllfv_cterm_cterm p_cterm)
+                             (upRen_cterm_cterm xi_cterm) s5
+                             match H with
+                             | conj _ H =>
+                                 match H with
+                                 | conj _ H =>
+                                     match H with
+                                     | conj _ H =>
+                                         match H with
+                                         | conj _ H =>
+                                             match H with
+                                             | conj _ H =>
+                                                 match H with
+                                                 | conj H _ => H
+                                                 end
+                                             end
+                                         end
+                                     end
+                                 end
+                             end)) I)))))
+  | clam s0 s1 s2 s3 =>
+      fun H =>
+      conj I
+        (conj
+           (allfvRenL_cterm p_cterm xi_cterm s1
+              match H with
+              | conj _ H => match H with
+                            | conj H _ => H
+                            end
+              end)
+           (conj
+              (allfvImpl_cterm _ _ (upAllfvRenL_cterm_cterm p_cterm xi_cterm)
+                 s2
+                 (allfvRenL_cterm (upAllfv_cterm_cterm p_cterm)
+                    (upRen_cterm_cterm xi_cterm) s2
+                    match H with
+                    | conj _ H =>
+                        match H with
+                        | conj _ H => match H with
+                                      | conj H _ => H
+                                      end
+                        end
+                    end))
+              (conj
+                 (allfvImpl_cterm _ _
+                    (upAllfvRenL_cterm_cterm p_cterm xi_cterm) s3
+                    (allfvRenL_cterm (upAllfv_cterm_cterm p_cterm)
+                       (upRen_cterm_cterm xi_cterm) s3
+                       match H with
+                       | conj _ H =>
+                           match H with
+                           | conj _ H =>
+                               match H with
+                               | conj _ H => match H with
+                                             | conj H _ => H
+                                             end
+                               end
+                           end
+                       end)) I)))
+  | capp s0 s1 =>
+      fun H =>
+      conj
+        (allfvRenL_cterm p_cterm xi_cterm s0 match H with
+                                             | conj H _ => H
+                                             end)
+        (conj
+           (allfvRenL_cterm p_cterm xi_cterm s1
+              match H with
+              | conj _ H => match H with
+                            | conj H _ => H
+                            end
+              end) I)
+  | cbot => fun H => I
+  | cbot_elim s0 s1 s2 =>
+      fun H =>
+      conj I
+        (conj
+           (allfvRenL_cterm p_cterm xi_cterm s1
+              match H with
+              | conj _ H => match H with
+                            | conj H _ => H
+                            end
+              end)
+           (conj
+              (allfvRenL_cterm p_cterm xi_cterm s2
+                 match H with
+                 | conj _ H =>
+                     match H with
+                     | conj _ H => match H with
+                                   | conj H _ => H
+                                   end
+                     end
+                 end) I))
+  end.
+
+Lemma upAllfvRenR_cterm_cterm (p : nat -> Prop) (xi : nat -> nat) :
+  forall x,
+  upAllfv_cterm_cterm (funcomp p xi) x ->
+  upAllfv_cterm_cterm p (upRen_cterm_cterm xi x).
+Proof.
+exact (fun x => match x with
+                | S n' => fun i => i
+                | O => fun H => H
+                end).
+Qed.
+
+Fixpoint allfvRenR_cterm (p_cterm : nat -> Prop) (xi_cterm : nat -> nat)
+(s : cterm) {struct s} :
+allfv_cterm (funcomp p_cterm xi_cterm) s ->
+allfv_cterm p_cterm (ren_cterm xi_cterm s) :=
+  match s with
+  | var s0 => fun H => H
+  | cSort s0 s1 => fun H => conj I (conj I I)
+  | cPi s0 s1 s2 s3 s4 s5 =>
+      fun H =>
+      conj I
+        (conj I
+           (conj I
+              (conj I
+                 (conj
+                    (allfvRenR_cterm p_cterm xi_cterm s4
+                       match H with
+                       | conj _ H =>
+                           match H with
+                           | conj _ H =>
+                               match H with
+                               | conj _ H =>
+                                   match H with
+                                   | conj _ H =>
+                                       match H with
+                                       | conj H _ => H
+                                       end
+                                   end
+                               end
+                           end
+                       end)
+                    (conj
+                       (allfvRenR_cterm (upAllfv_cterm_cterm p_cterm)
+                          (upRen_cterm_cterm xi_cterm) s5
+                          (allfvImpl_cterm _ _
+                             (upAllfvRenR_cterm_cterm p_cterm xi_cterm) s5
+                             match H with
+                             | conj _ H =>
+                                 match H with
+                                 | conj _ H =>
+                                     match H with
+                                     | conj _ H =>
+                                         match H with
+                                         | conj _ H =>
+                                             match H with
+                                             | conj _ H =>
+                                                 match H with
+                                                 | conj H _ => H
+                                                 end
+                                             end
+                                         end
+                                     end
+                                 end
+                             end)) I)))))
+  | clam s0 s1 s2 s3 =>
+      fun H =>
+      conj I
+        (conj
+           (allfvRenR_cterm p_cterm xi_cterm s1
+              match H with
+              | conj _ H => match H with
+                            | conj H _ => H
+                            end
+              end)
+           (conj
+              (allfvRenR_cterm (upAllfv_cterm_cterm p_cterm)
+                 (upRen_cterm_cterm xi_cterm) s2
+                 (allfvImpl_cterm _ _
+                    (upAllfvRenR_cterm_cterm p_cterm xi_cterm) s2
+                    match H with
+                    | conj _ H =>
+                        match H with
+                        | conj _ H => match H with
+                                      | conj H _ => H
+                                      end
+                        end
+                    end))
+              (conj
+                 (allfvRenR_cterm (upAllfv_cterm_cterm p_cterm)
+                    (upRen_cterm_cterm xi_cterm) s3
+                    (allfvImpl_cterm _ _
+                       (upAllfvRenR_cterm_cterm p_cterm xi_cterm) s3
+                       match H with
+                       | conj _ H =>
+                           match H with
+                           | conj _ H =>
+                               match H with
+                               | conj _ H => match H with
+                                             | conj H _ => H
+                                             end
+                               end
+                           end
+                       end)) I)))
+  | capp s0 s1 =>
+      fun H =>
+      conj
+        (allfvRenR_cterm p_cterm xi_cterm s0 match H with
+                                             | conj H _ => H
+                                             end)
+        (conj
+           (allfvRenR_cterm p_cterm xi_cterm s1
+              match H with
+              | conj _ H => match H with
+                            | conj H _ => H
+                            end
+              end) I)
+  | cbot => fun H => I
+  | cbot_elim s0 s1 s2 =>
+      fun H =>
+      conj I
+        (conj
+           (allfvRenR_cterm p_cterm xi_cterm s1
+              match H with
+              | conj _ H => match H with
+                            | conj H _ => H
+                            end
+              end)
+           (conj
+              (allfvRenR_cterm p_cterm xi_cterm s2
+                 match H with
+                 | conj _ H =>
+                     match H with
+                     | conj _ H => match H with
+                                   | conj H _ => H
+                                   end
+                     end
+                 end) I))
+  end.
+
+End Allfv.
+
+Module Extra.
+
+Import Core.
+
+#[global]Hint Opaque subst_cterm: rewrite.
+
+#[global]Hint Opaque ren_cterm: rewrite.
+
+End Extra.
+
+Module interface.
+
+Export Core.
+
+Export Allfv.
+
+Export Extra.
+
+End interface.
+
+Export interface.
+
